Weidenbach_Book/IsaSAT_Restart_Heuristics_SML.thy
@@ -255,6 +255,44 @@ sepref_definition (in -) clause_score_extract_code
   by sepref
 
 declare clause_score_extract_code.refine[sepref_fr_rules]
+(*TODO Move*)
+sepref_definition isa_get_clause_LBD_code2
+  is \<open>uncurry isa_get_clause_LBD\<close>
+  :: \<open>(arl64_assn uint32_assn)\<^sup>k *\<^sub>a nat_assn\<^sup>k \<rightarrow>\<^sub>a uint32_assn\<close>
+  unfolding isa_get_clause_LBD_def fast_minus_def[symmetric]
+  by sepref
+
+lemma isa_get_clause_LBD_code[sepref_fr_rules]:
+  \<open>(uncurry isa_get_clause_LBD_code2, uncurry (RETURN \<circ>\<circ> get_clause_LBD))
+     \<in> [uncurry get_clause_LBD_pre]\<^sub>a arena_fast_assn\<^sup>k *\<^sub>a nat_assn\<^sup>k \<rightarrow> uint32_nat_assn\<close>
+  using isa_get_clause_LBD_code2.refine[FCOMP isa_get_clause_LBD_get_clause_LBD[unfolded convert_fref]]
+  unfolding hr_comp_assoc[symmetric] list_rel_compp status_assn_alt_def uncurry_def
+  by (auto simp add: arl64_assn_comp update_lbd_pre_def)
+sepref_definition isa_arena_act_code2
+  is \<open>uncurry isa_arena_act\<close>
+  :: \<open>(arl64_assn uint32_assn)\<^sup>k *\<^sub>a nat_assn\<^sup>k \<rightarrow>\<^sub>a uint32_assn\<close>
+  unfolding isa_arena_act_def ACTIVITY_SHIFT_def fast_minus_def[symmetric]
+  by sepref
+
+lemma isa_arena_act_code2[sepref_fr_rules]:
+  \<open>(uncurry isa_arena_act_code2, uncurry (RETURN \<circ>\<circ> arena_act))
+     \<in> [uncurry arena_act_pre]\<^sub>a arena_fast_assn\<^sup>k *\<^sub>a nat_assn\<^sup>k \<rightarrow> uint32_nat_assn\<close>
+  using isa_arena_act_code2.refine[FCOMP isa_arena_act_arena_act[unfolded convert_fref]]
+  unfolding hr_comp_assoc[symmetric] list_rel_compp status_assn_alt_def uncurry_def
+  by (auto simp add: arl64_assn_comp update_lbd_pre_def)
+
+(*END Move*)
+find_theorems arena_act
+thm isa_arena_act_code
+sepref_definition (in -) clause_score_extract_fast_code
+  is \<open>uncurry (RETURN oo clause_score_extract)\<close>
+  :: \<open>[uncurry valid_sort_clause_score_pre_at]\<^sub>a
+      arena_fast_assn\<^sup>k *\<^sub>a nat_assn\<^sup>k \<rightarrow> uint32_nat_assn *a uint32_nat_assn\<close>
+  supply uint32_max_uint32_nat_assn[sepref_fr_rules]
+  unfolding clause_score_extract_def insert_sort_inner_def valid_sort_clause_score_pre_at_def
+  by sepref
+
+declare clause_score_extract_fast_code.refine[sepref_fr_rules]
 
 
 sepref_definition (in -) partition_main_clause_code
@@ -270,7 +308,7 @@ sepref_definition (in -) partition_main_clause_code
 sepref_definition (in -) partition_main_clause_fast_code
   is \<open>uncurry3 partition_main_clause\<close>
   :: \<open>[\<lambda>(((arena, i), j), vdom). length vdom \<le> uint64_max \<and> valid_sort_clause_score_pre arena vdom]\<^sub>a
-      arena_assn\<^sup>k *\<^sub>a uint64_nat_assn\<^sup>k *\<^sub>a uint64_nat_assn\<^sup>k *\<^sub>a vdom_assn\<^sup>d \<rightarrow> vdom_assn *a uint64_nat_assn\<close>
+      arena_fast_assn\<^sup>k *\<^sub>a uint64_nat_assn\<^sup>k *\<^sub>a uint64_nat_assn\<^sup>k *\<^sub>a vdom_assn\<^sup>d \<rightarrow> vdom_assn *a uint64_nat_assn\<close>
   supply insort_inner_clauses_by_score_invI[intro] [[goals_limit=1]]
     partition_main_inv_def[simp] mset_eq_length[dest]
   unfolding partition_main_clause_def partition_between_ref_def
@@ -301,13 +339,14 @@ lemma div2_hnr[sepref_fr_rules]: \<open>(return o (\<lambda>n. n >> 1), RETURN o
 sepref_definition (in -) partition_clause_fast_code
   is \<open>uncurry3 partition_clause\<close>
   :: \<open>[\<lambda>(((arena, i), j), vdom). length vdom \<le> uint64_max \<and> valid_sort_clause_score_pre arena vdom]\<^sub>a
-      arena_assn\<^sup>k *\<^sub>a uint64_nat_assn\<^sup>k *\<^sub>a uint64_nat_assn\<^sup>k *\<^sub>a vdom_assn\<^sup>d \<rightarrow> vdom_assn *a uint64_nat_assn\<close>
+      arena_fast_assn\<^sup>k *\<^sub>a uint64_nat_assn\<^sup>k *\<^sub>a uint64_nat_assn\<^sup>k *\<^sub>a vdom_assn\<^sup>d \<rightarrow> vdom_assn *a uint64_nat_assn\<close>
   supply insort_inner_clauses_by_score_invI[intro] valid_sort_clause_score_pre_swap[
     unfolded WB_More_Refinement_List.swap_def IICF_List.swap_def[symmetric], intro] mset_eq_length[dest]
   unfolding partition_clause_def partition_between_ref_def div2_def[symmetric]
     choose_pivot3_def partition_main_clause_def[symmetric]
     WB_More_Refinement_List.swap_def IICF_List.swap_def[symmetric]
   by sepref
+
 
 declare partition_clause_code.refine[sepref_fr_rules]
   partition_clause_fast_code.refine[sepref_fr_rules]
@@ -335,7 +374,7 @@ lemma minus_uint64_safe:
 sepref_definition (in -) sort_clauses_by_score_fast_code
   is \<open>uncurry quicksort_clauses_by_score\<close>
   :: \<open>[\<lambda>(arena, vdom). length vdom \<le> uint64_max \<and> valid_sort_clause_score_pre arena vdom]\<^sub>a
-      arena_assn\<^sup>k *\<^sub>a vdom_assn\<^sup>d \<rightarrow> vdom_assn\<close>
+      arena_fast_assn\<^sup>k *\<^sub>a vdom_assn\<^sup>d \<rightarrow> vdom_assn\<close>
   supply sort_clauses_by_score_invI[intro] [[goals_limit=1]] mset_eq_length[dest] minus_uint64_safe[sepref_fr_rules]
   unfolding insert_sort_def
     quicksort_clauses_by_score_def
@@ -543,17 +582,45 @@ sepref_definition isasat_replace_annot_in_trail_slow_code
 (*TODO Move*)
 sepref_definition mark_garbage_fast_code
   is \<open>uncurry mark_garbage\<close>
-  :: \<open>(arl_assn uint32_assn)\<^sup>d *\<^sub>a uint64_nat_assn\<^sup>k \<rightarrow>\<^sub>a arl_assn uint32_assn\<close>
+  :: \<open>(arl64_assn uint32_assn)\<^sup>d *\<^sub>a uint64_nat_assn\<^sup>k \<rightarrow>\<^sub>a arl64_assn uint32_assn\<close>
   supply STATUS_SHIFT_hnr[sepref_fr_rules]
   unfolding mark_garbage_def fast_minus_def[symmetric]
   by sepref
 
 lemma mark_garbage_fast_hnr[sepref_fr_rules]:
   \<open>(uncurry mark_garbage_fast_code, uncurry (RETURN oo extra_information_mark_to_delete))
-  \<in> [mark_garbage_pre]\<^sub>a  arena_assn\<^sup>d *\<^sub>a uint64_nat_assn\<^sup>k \<rightarrow> arena_assn\<close>
+  \<in> [mark_garbage_pre]\<^sub>a  arena_fast_assn\<^sup>d *\<^sub>a uint64_nat_assn\<^sup>k \<rightarrow> arena_fast_assn\<close>
   using mark_garbage_fast_code.refine[FCOMP isa_mark_garbage[unfolded convert_fref]]
   unfolding hr_comp_assoc[symmetric] list_rel_compp status_assn_alt_def uncurry_def
-  by (auto simp add: arl_assn_comp update_lbd_pre_def)
+  by (auto simp add: arl64_assn_comp update_lbd_pre_def)
+
+context
+  notes [fcomp_norm_unfold] = arl64_assn_def[symmetric] arl64_assn_comp'
+  notes [intro!] = hfrefI hn_refineI[THEN hn_refine_preI]
+  notes [simp] = pure_def hn_ctxt_def invalid_assn_def
+begin
+definition arl64_set_nat :: "'a::heap array_list64 \<Rightarrow> nat \<Rightarrow> 'a \<Rightarrow> 'a array_list64 Heap" where
+  "arl64_set_nat \<equiv> \<lambda>(a,n) i x. do { a \<leftarrow> Array.upd i x a; return (a,n)}"
+
+  lemma arl64_set_hnr_aux: "(uncurry2 arl64_set_nat,uncurry2 (RETURN ooo op_list_set)) \<in> [\<lambda>((l,i),_). i<length l]\<^sub>a (is_array_list64\<^sup>d *\<^sub>a nat_assn\<^sup>k *\<^sub>a id_assn\<^sup>k) \<rightarrow> is_array_list64"
+    by (sep_auto simp: arl64_set_nat_def is_array_list64_def)
+  sepref_decl_impl arl64_set_nat: arl64_set_hnr_aux .
+
+end
+
+sepref_definition mark_garbage_fast_code2
+  is \<open>uncurry mark_garbage\<close>
+  :: \<open>(arl64_assn uint32_assn)\<^sup>d *\<^sub>a nat_assn\<^sup>k \<rightarrow>\<^sub>a arl64_assn uint32_assn\<close>
+  unfolding STATUS_SHIFT_def
+  unfolding mark_garbage_def fast_minus_def[symmetric]
+  by sepref
+
+lemma mark_garbage_fast_hnr2[sepref_fr_rules]:
+  \<open>(uncurry mark_garbage_fast_code2, uncurry (RETURN oo extra_information_mark_to_delete))
+  \<in> [mark_garbage_pre]\<^sub>a  arena_fast_assn\<^sup>d *\<^sub>a nat_assn\<^sup>k \<rightarrow> arena_fast_assn\<close>
+  using mark_garbage_fast_code2.refine[FCOMP isa_mark_garbage[unfolded convert_fref]]
+  unfolding hr_comp_assoc[symmetric] list_rel_compp status_assn_alt_def uncurry_def
+  by (auto simp add: arl64_assn_comp)
 (*END Move*)
 
 sepref_register mark_garbage_heur2
@@ -666,19 +733,21 @@ sepref_definition remove_one_annot_true_clause_imp_wl_D_heur_slow_code
 declare remove_one_annot_true_clause_imp_wl_D_heur_code.refine[sepref_fr_rules]
    remove_one_annot_true_clause_imp_wl_D_heur_slow_code.refine[sepref_fr_rules]
 
+declare fm_mv_clause_to_new_arena_fast_code.refine[sepref_fr_rules]
 sepref_definition isasat_GC_clauses_prog_copy_wl_entry_code
   is \<open>uncurry3 isasat_GC_clauses_prog_copy_wl_entry\<close>
   :: \<open>[\<lambda>(((N, _), _), _). length N \<le> uint64_max]\<^sub>a
-     arena_assn\<^sup>d *\<^sub>a watchlist_fast_assn\<^sup>k *\<^sub>a unat_lit_assn\<^sup>k *\<^sub>a (arena_assn *a vdom_assn *a vdom_assn)\<^sup>d \<rightarrow>
-     (arena_assn *a (arena_assn *a vdom_assn *a vdom_assn))\<close>
-  supply [[goals_limit=1]] Pos_unat_lit_assn'[sepref_fr_rules] length_ll_def[simp]
+     arena_fast_assn\<^sup>d *\<^sub>a watchlist_fast_assn\<^sup>k *\<^sub>a unat_lit_assn\<^sup>k *\<^sub>a
+         (arena_fast_assn *a vdom_assn *a vdom_assn)\<^sup>d \<rightarrow>
+     (arena_fast_assn *a (arena_fast_assn *a vdom_assn *a vdom_assn))\<close>
+  supply [[goals_limit=1]] Pos_unat_lit_assn'[sepref_fr_rules] length_ll_def[simp] if_splits[split]
   unfolding isasat_GC_clauses_prog_copy_wl_entry_def nth_rll_def[symmetric]
     length_ll_def[symmetric] zero_uint64_nat_def[symmetric] one_uint64_nat_def[symmetric]
-  apply (rewrite at \<open>If (\<hole> < _)\<close> four_uint64_nat_def[symmetric])
-  apply (rewrite at \<open>fm_mv_clause_to_new_arena \<hole>\<close> nat_of_uint64_conv_def[symmetric])
+    four_uint64_nat_def[symmetric] five_uint64_nat_def[symmetric]
   apply (rewrite at \<open>let _ = length_ll _ \<hole> in _\<close> uint64_of_uint32_conv_def[symmetric])
+  apply (rewrite at \<open>_ @ [\<hole>]\<close> nat_of_uint64_conv_def[symmetric])
+  apply (rewrite at \<open>If _ (_ @ [\<hole>])\<close> nat_of_uint64_conv_def[symmetric])
   by sepref
-
 
 sepref_definition isasat_GC_clauses_prog_copy_wl_entry_slow_code
   is \<open>uncurry3 isasat_GC_clauses_prog_copy_wl_entry\<close>
@@ -687,7 +756,7 @@ sepref_definition isasat_GC_clauses_prog_copy_wl_entry_slow_code
   supply [[goals_limit=1]] Pos_unat_lit_assn'[sepref_fr_rules] length_ll_def[simp]
   unfolding isasat_GC_clauses_prog_copy_wl_entry_def nth_rll_def[symmetric]
     length_ll_def[symmetric]
-  apply (rewrite at \<open>If (\<hole> < _)\<close> four_uint64_nat_def[symmetric])
+  apply (rewrite at \<open>let _ = _ + (If (\<hole> < _) _ _) in _\<close> four_uint64_nat_def[symmetric])
   by sepref
 
 
@@ -705,8 +774,8 @@ lemma length_shorten_take_ll[simp]: \<open>length (shorten_take_ll a j W) = leng
 sepref_definition isasat_GC_clauses_prog_single_wl_code
   is \<open>uncurry3 isasat_GC_clauses_prog_single_wl\<close>
   :: \<open>[\<lambda>(((N, _), _), A). A \<le> uint32_max div 2 \<and> length N \<le> uint64_max]\<^sub>a
-     arena_assn\<^sup>d *\<^sub>a (arena_assn *a vdom_assn *a vdom_assn)\<^sup>d *\<^sub>a watchlist_fast_assn\<^sup>d *\<^sub>a uint32_nat_assn\<^sup>k \<rightarrow>
-     (arena_assn *a (arena_assn *a vdom_assn *a vdom_assn) *a watchlist_fast_assn)\<close>
+     arena_fast_assn\<^sup>d *\<^sub>a (arena_fast_assn *a vdom_assn *a vdom_assn)\<^sup>d *\<^sub>a watchlist_fast_assn\<^sup>d *\<^sub>a uint32_nat_assn\<^sup>k \<rightarrow>
+     (arena_fast_assn *a (arena_fast_assn *a vdom_assn *a vdom_assn) *a watchlist_fast_assn)\<close>
   supply [[goals_limit=1]] Pos_unat_lit_assn'[sepref_fr_rules]
   unfolding isasat_GC_clauses_prog_single_wl_def zero_uint64_nat_def[symmetric]
     shorten_take_ll_0[symmetric]
@@ -736,8 +805,8 @@ sepref_definition isasat_GC_clauses_prog_wl2_code
   is \<open>uncurry2 isasat_GC_clauses_prog_wl2'\<close>
   :: \<open>[\<lambda>((_, _), (N, _)). length N \<le> uint64_max]\<^sub>a
      (array_assn vmtf_node_assn)\<^sup>k *\<^sub>a (option_assn uint32_nat_assn)\<^sup>k *\<^sub>a 
-     (arena_assn *a (arena_assn *a vdom_assn *a vdom_assn) *a watchlist_fast_assn)\<^sup>d \<rightarrow>
-     (arena_assn *a (arena_assn *a vdom_assn *a vdom_assn) *a watchlist_fast_assn)\<close>
+     (arena_fast_assn *a (arena_fast_assn *a vdom_assn *a vdom_assn) *a watchlist_fast_assn)\<^sup>d \<rightarrow>
+     (arena_fast_assn *a (arena_fast_assn *a vdom_assn *a vdom_assn) *a watchlist_fast_assn)\<close>
   supply [[goals_limit=1]]
   unfolding isasat_GC_clauses_prog_wl2_def isasat_GC_clauses_prog_wl2'_def
   by sepref
@@ -754,6 +823,14 @@ sepref_definition isasat_GC_clauses_prog_wl2_slow_code
 declare isasat_GC_clauses_prog_wl2_code.refine[sepref_fr_rules]
    isasat_GC_clauses_prog_wl2_slow_code.refine[sepref_fr_rules]
 
+(*TODO Move replace*)
+lemma arl64_take[sepref_fr_rules]:
+  \<open>(uncurry (return oo arl64_take), uncurry (RETURN oo take)) \<in>
+    [\<lambda>(n, xs). n \<le> length xs]\<^sub>a uint64_nat_assn\<^sup>k *\<^sub>a (arl64_assn R)\<^sup>d \<rightarrow> arl64_assn R\<close>
+  by (sepref_to_hoare)
+    (sep_auto simp: arl64_assn_def arl64_take_def is_array_list64_def hr_comp_def
+      uint64_nat_rel_def br_def list_rel_def list_all2_conv_all_nth)
+
 sepref_register isasat_GC_clauses_prog_wl isasat_GC_clauses_prog_wl2' rewatch_heur_st
 sepref_definition isasat_GC_clauses_prog_wl_code
   is \<open>isasat_GC_clauses_prog_wl\<close>
@@ -761,6 +838,7 @@ sepref_definition isasat_GC_clauses_prog_wl_code
   supply [[goals_limit=1]]
   unfolding isasat_GC_clauses_prog_wl_def isasat_bounded_assn_def
      isasat_GC_clauses_prog_wl2'_def[symmetric]
+  apply (rewrite in \<open>(_, _, _, _, _, take \<hole> _)\<close> zero_uint64_nat_def[symmetric])
   by sepref
 
 sepref_definition isasat_GC_clauses_prog_wl_slow_code
@@ -771,6 +849,22 @@ sepref_definition isasat_GC_clauses_prog_wl_slow_code
     IICF_Array_List.arl.fold_custom_empty isasat_GC_clauses_prog_wl2'_def[symmetric]
   by sepref
 
+(*TODO Move*)
+sepref_definition isa_arena_length_fast_code2
+  is \<open>uncurry isa_arena_length\<close>
+  :: \<open>(arl64_assn uint32_assn)\<^sup>k *\<^sub>a nat_assn\<^sup>k \<rightarrow>\<^sub>a uint64_assn\<close>
+  supply arena_el_assn_alt_def[symmetric, simp] sum_uint64_assn[sepref_fr_rules]
+    minus_uint64_nat_assn[sepref_fr_rules]
+  unfolding isa_arena_length_def SIZE_SHIFT_def fast_minus_def
+  by sepref
+
+lemma isa_arena_length_fast_code2_refine[sepref_fr_rules]:
+  \<open>(uncurry isa_arena_length_fast_code2, uncurry (RETURN \<circ>\<circ> arena_length))
+  \<in> [uncurry arena_is_valid_clause_idx]\<^sub>a
+    arena_fast_assn\<^sup>k *\<^sub>a nat_assn\<^sup>k \<rightarrow> uint64_nat_assn\<close>
+  using isa_arena_length_fast_code2.refine[FCOMP isa_arena_length_arena_length[unfolded convert_fref]]
+  unfolding hr_comp_assoc[symmetric] uncurry_def list_rel_compp
+  by (simp add: arl64_assn_comp)
 
 sepref_definition rewatch_heur_st_code
   is \<open>rewatch_heur_st\<close>
