Weidenbach_Book/IsaSAT_Clauses_SML.thy
@@ -183,10 +183,11 @@ sepref_definition append_and_length_code
    two_uint64_nat_def[symmetric]
    apply (rewrite in \<open>let _ = _ - _ in _\<close> length_uint64_nat_def[symmetric])
    apply (rewrite in \<open>let _ = _ in let _ = _ in let _ = \<hole> in _\<close> uint32_of_uint64_conv_def[symmetric])
-   apply (rewrite in \<open>_ < length _\<close> length_uint64_nat_def[symmetric])
+   apply (rewrite at \<open>WHILEIT _ (\<lambda>(_, _)._ < \<hole>)\<close> length_uint64_nat_def[symmetric])
   by sepref
 
 declare append_and_length_code.refine[sepref_fr_rules]
+
 
 sepref_definition (in -) header_size_fast_code
   is \<open>RETURN o header_size\<close>
@@ -215,21 +216,21 @@ sepref_definition (in -) header_size_fast_code
 declare (in -)header_size_fast_code.refine[sepref_fr_rules]
 (* End Move *)
 
+
 sepref_definition (in -)append_and_length_fast_code
   is \<open>uncurry2 fm_add_new_fast\<close>
   :: \<open>[append_and_length_fast_code_pre]\<^sub>a
-     bool_assn\<^sup>k *\<^sub>a clause_ll_assn\<^sup>d *\<^sub>a (arena_assn)\<^sup>d \<rightarrow>
-       arena_assn *a uint64_nat_assn\<close>
+     bool_assn\<^sup>k *\<^sub>a clause_ll_assn\<^sup>d *\<^sub>a (arena_fast_assn)\<^sup>d \<rightarrow>
+       arena_fast_assn *a uint64_nat_assn\<close>
   supply [[goals_limit=1]] le_uint32_max_le_uint64_max[intro] append_and_length_code_fast[intro]
-    header_size_def[simp]
+    header_size_def[simp] if_splits[split] header_size_fast_code.refine[sepref_fr_rules]
   unfolding fm_add_new_def AStatus_IRRED_def[symmetric] append_and_length_fast_code_pre_def
    AStatus_LEARNED_def[symmetric] AStatus_LEARNED2_def[symmetric]
-   AStatus_IRRED2_def[symmetric]
+   AStatus_IRRED2_def[symmetric]  four_uint64_nat_def[symmetric]
    two_uint64_nat_def[symmetric] fm_add_new_fast_def
    apply (rewrite in \<open>let _ = _ - _ in _\<close> length_uint64_nat_def[symmetric])
-   apply (rewrite in \<open>let _ = _ in _\<close> length_uint64_nat_def[symmetric])
    apply (rewrite in \<open>let _ = _ in let _ = _ in let _ = \<hole> in _\<close> uint32_of_uint64_conv_def[symmetric])
-  apply (rewrite in \<open>_ < length _\<close> length_uint64_nat_def[symmetric])
+  apply (rewrite at \<open>WHILEIT _ (\<lambda>(_, _)._ < \<hole>)\<close> length_uint64_nat_def[symmetric])
   by sepref
 
 declare append_and_length_fast_code.refine[sepref_fr_rules]
@@ -273,8 +274,8 @@ lemma swap_lits_refine[sepref_fr_rules]:
 sepref_definition (in -) swap_lits_fast_code
   is \<open>uncurry3 isa_arena_swap\<close>
   :: \<open>[\<lambda>(((_, _), _), N). length N \<le> uint64_max]\<^sub>a
-      uint64_nat_assn\<^sup>k *\<^sub>a uint64_nat_assn\<^sup>k *\<^sub>a uint64_nat_assn\<^sup>k *\<^sub>a (arl_assn uint32_assn)\<^sup>d  \<rightarrow>
-         arl_assn uint32_assn\<close>
+      uint64_nat_assn\<^sup>k *\<^sub>a uint64_nat_assn\<^sup>k *\<^sub>a uint64_nat_assn\<^sup>k *\<^sub>a (arl64_assn uint32_assn)\<^sup>d  \<rightarrow>
+         arl64_assn uint32_assn\<close>
   unfolding isa_arena_swap_def WB_More_Refinement_List.swap_def IICF_List.swap_def[symmetric]
   by sepref
 
@@ -282,10 +283,10 @@ sepref_definition (in -) swap_lits_fast_code
 lemma swap_lits_fast_refine[sepref_fr_rules]:
   \<open>(uncurry3 swap_lits_fast_code, uncurry3 (RETURN oooo swap_lits))
   \<in> [\<lambda>(((C, i), j), arena). swap_lits_pre C i j arena \<and> length arena \<le> uint64_max]\<^sub>a
-     uint64_nat_assn\<^sup>k *\<^sub>a uint64_nat_assn\<^sup>k *\<^sub>a uint64_nat_assn\<^sup>k *\<^sub>a arena_assn\<^sup>d \<rightarrow> arena_assn\<close>
+     uint64_nat_assn\<^sup>k *\<^sub>a uint64_nat_assn\<^sup>k *\<^sub>a uint64_nat_assn\<^sup>k *\<^sub>a arena_fast_assn\<^sup>d \<rightarrow> arena_fast_assn\<close>
   using swap_lits_fast_code.refine[FCOMP isa_arena_swap[unfolded convert_fref]]
   unfolding hr_comp_assoc[symmetric] list_rel_compp status_assn_alt_def uncurry_def
-  by (auto simp add: arl_assn_comp)
+  by (auto simp add: arl64_assn_comp)
 
 declare swap_lits_fast_code.refine[sepref_fr_rules]
 sepref_definition fm_mv_clause_to_new_arena_code
@@ -293,6 +294,17 @@ sepref_definition fm_mv_clause_to_new_arena_code
   :: \<open>nat_assn\<^sup>k *\<^sub>a arena_assn\<^sup>k *\<^sub>a arena_assn\<^sup>d \<rightarrow>\<^sub>a arena_assn\<close>
   supply [[goals_limit=1]]
   unfolding fm_mv_clause_to_new_arena_def
+  by sepref
+
+declare fm_mv_clause_to_new_arena_code.refine[sepref_fr_rules]
+sepref_definition fm_mv_clause_to_new_arena_fast_code
+  is \<open>uncurry2 fm_mv_clause_to_new_arena\<close>
+  :: \<open>[\<lambda>((n, arena\<^sub>o), arena). length arena\<^sub>o \<le> uint64_max \<and> length arena + arena_length arena\<^sub>o n +
+         (if arena_length arena\<^sub>o  n \<le> 4 then 4 else 5) \<le> uint64_max]\<^sub>a
+       uint64_nat_assn\<^sup>k *\<^sub>a arena_fast_assn\<^sup>k *\<^sub>a arena_fast_assn\<^sup>d \<rightarrow> arena_fast_assn\<close>
+  supply [[goals_limit=1]] if_splits[split]
+  unfolding fm_mv_clause_to_new_arena_def four_uint64_nat_def[symmetric] five_uint64_nat_def[symmetric]
+    one_uint64_nat_def[symmetric] nat_of_uint64_conv_def
   by sepref
 
 declare fm_mv_clause_to_new_arena_code.refine[sepref_fr_rules]
